figured out how to define FunInput, FunOutput, and funElem in a way that we can convert funElems into FxInterps

theories/Ref/TpDesc.v
@@ -414,6 +414,7 @@ Fixpoint TpFunInput env (T:TpDesc) : Type@{entree_u} :=
   | _ => Empty_set
   end.
 
+(* The output type of a monadic function of type T with the given inputs *)
 Fixpoint TpFunOutput {env T} : TpFunInput env T -> Type@{entree_u} :=
   match T return TpFunInput env T -> Type with
   | Tp_M R => fun _ => tpElem nil (tpSubst 0 env R)
@@ -422,48 +423,13 @@ Fixpoint TpFunOutput {env T} : TpFunInput env T -> Type@{entree_u} :=
   | _ => fun _ => Empty_set
   end.
 
-(* We build an IsTpDesc instance for each environment, though we only want to
-use the empty environment for "the" instance *)
-Definition IsTpDescInEnv env : IsTpDesc TpDesc :=
-  {|
-    FunInput := @TpFunInput env;
-    FunOutput := @TpFunOutput env;
-    dec_eq_Tp := dec_eq_TpDesc
-  |}.
-
-Global Instance IsTpDesc_TpDesc : IsTpDesc TpDesc := IsTpDescInEnv nil.
-
-
-(*
-FIXME: I think this is the wrong approach, but keeping it around just in case
-
-(* A tuple of inputs to a functional type description; NOTE: we define this as
-an inductive type, rather than a function on TpDescs, so we can perform the type
-substitution in the Tp_Pi case *)
-Inductive TpFunInput : TpDesc -> Type@{entree_u} :=
-| TpFunInput_M R : TpFunInput (Tp_M R)
-| TpFunInput_Pi K B (elem: kindElem K) (args: TpFunInput (tpSubst1 elem B)) :
-  TpFunInput (Tp_Pi K B)
-| TpFunInput_Arr A B (arg: tpElem nil A) (args: TpFunInput B) :
-  TpFunInput (Tp_Arr A B)
-.
-
-(* The output type of a function applied to the given inputs *)
-Fixpoint TpFunOutput {T} (args: TpFunInput T) : Type@{entree_u} :=
-  match args in TpFunInput T return Type with
-  | TpFunInput_M R => tpElem nil R
-  | TpFunInput_Pi K B elem args' => TpFunOutput args'
-  | TpFunInput_Arr A B arg args' => TpFunOutput args'
-  end.
-
+(* The above define input and output function types for TpDescs *)
 Global Instance IsTpDesc_TpDesc : IsTpDesc TpDesc :=
   {|
-    FunInput := TpFunInput;
-    FunOutput := @TpFunOutput;
+    FunInput := @TpFunInput nil;
+    FunOutput := @TpFunOutput nil;
     dec_eq_Tp := dec_eq_TpDesc
   |}.
-
-*)
 
 (* A monadic function of a given type description *)
 Fixpoint funElem (E:EvType) env T : Type@{entree_u} :=
@@ -474,12 +440,22 @@ Fixpoint funElem (E:EvType) env T : Type@{entree_u} :=
   | _ => Empty_set
   end.
 
-(* Convert a monadic function to an FxInterp *)
-Fixpoint funElemToInterp {E env T} : funElem E env T ->
-                                     @FxInterp TpDesc _ E T :=
-  match T return funElem E env T -> @FxInterp TpDesc _ E T with
-  | Tp_M R => fun elem _ => elem
+(* Convert a monadic function to an FxInterp relative to an environment *)
+Fixpoint funElemToInterpEnv {E env T} : funElem E env T ->
+                                        forall args:TpFunInput env T,
+                                          fixtree TpDesc E (TpFunOutput args) :=
+  match T return funElem E env T ->
+                 forall args:TpFunInput env T,
+                   fixtree TpDesc E (TpFunOutput args) with
+  | Tp_M R => fun m _ => m
+  | Tp_Pi K B => fun f args => funElemToInterpEnv (f (projT1 args)) (projT2 args)
+  | Tp_Arr A B => fun f args => funElemToInterpEnv (f (fst args)) (snd args)
+  | _ => fun (v:Empty_set) => match v with end
   end.
+
+(* Convert a monadic function to an FxInterp in the top-level environment *)
+Definition funElemToInterp {E T} : funElem E nil T -> @FxInterp TpDesc _ E T :=
+  funElemToInterpEnv.
 
 
 End TpDesc.
